Stronger abstraction separation

coq/assoc_spec.v
@@ -7,10 +7,12 @@ Local Open Scope Z_scope.
 (*Local Open Scope Z.*)
 Locate Z.
 
-Function arrPut (arr:Z -> Z) (k:Z) (v:Z) : Z -> Z :=
+Definition ArrayZ := Z->Z.
+
+Function arrPut (arr: ArrayZ) (k:Z) (v:Z) : Z -> Z :=
   fun (kk:Z) => if (Z.eq_dec k kk) then v else arr kk.
 
-Function arrGet (arr:Z -> Z) (k:Z) : Z :=
+Function arrGet (arr: ArrayZ) (k:Z) : Z :=
   arr k.
 
 Lemma getput1: forall arr k v, arrGet (arrPut arr k v) k = v.
@@ -20,11 +22,11 @@ unfold arrGet, arrPut.
 destruct Z.eq_dec;[auto|tauto].
 Qed.
 
-Lemma getput2: forall arr k1 k2 v1 v2, arr k1 = v1 ->
-                                       k1 <> k2 -> arrGet (arrPut arr k2 v2) k1 = v1.
+Lemma getput2: forall arr k1 k2 v2, k2 <> k1 -> arrGet (arrPut arr k2 v2) k1 = 
+                                                arrGet arr k1.
 Proof.
 intros.
 unfold arrGet, arrPut.
-destruct Z.eq_dec;[symmetry in e;contradiction|assumption].
+destruct Z.eq_dec;[contradiction|tauto].
 Qed.
 
